first

src/Distributions/Geometric/Model.dfy
@@ -5,10 +5,12 @@
 
 include "../../ProbabilisticProgramming/Monad.dfy"
 include "../../ProbabilisticProgramming/WhileAndUntil.dfy"
+include "../../ProbabilisticProgramming/Independence.dfy"
 include "Correctness.dfy"
 
 import opened Monad
 import opened WhileAndUntil
+import opened Independence
 
 // Equation (4.18)
 function ProbGeometric(): Hurd<int> {
@@ -19,9 +21,21 @@ function ProbGeometric(): Hurd<int> {
   Bind(g, f)
 }
 
-  // Equation (4.17)
+// Equation (4.17)
 function ProbGeometricIter(t: (bool, int)): (f: Hurd<(bool, int)>)
   ensures forall s :: f(s) == ((Head(s), t.1 + 1), Tail(s))
+  ensures IsIndepFn(f)
 {
-  Bind(Deconstruct, (b': bool) => Return((b', t.1 + 1)))
+  var g := (b': bool) => Return((b', t.1 + 1));
+  assert forall b' :: IsIndepFn(g(b')) by {
+    forall b' ensures IsIndepFn(g(b')) {
+      ReturnIsIndepFn((b', t.1 + 1));
+    }
+  }
+  var f := Bind(Deconstruct, g);
+  assert IsIndepFn(f) by {
+    DeconstructIsIndepFn();
+    IndepFnIsCompositional(Deconstruct, g);
+  }
+  f
 }
